'EvalToSet' 까지는 다 했고...이제 'Notation' 만이 남았다!

Nemonuri/Executions/ExecutionFragment/Expr/Basic.lean
@@ -17,10 +17,19 @@ inductive IsPrefixFragment : ts.FiniteExecutionFragmentRaw → Prop where
           (req: ts.IsFiniteExecutionFragment ⟨states ++ [stateLast], actions⟩)
           : IsPrefixFragment ⟨states ++ [stateLast], actions⟩
 
-inductive IsPostfixFragment : ts.FiniteExecutionFragmentRaw → Prop where
+inductive IsSuffixFragment : ts.FiniteExecutionFragmentRaw → Prop where
   | intro (states: List ts.S) (actions: List ts.Act) (state0: ts.S)
           (req: ts.IsFiniteExecutionFragment ⟨state0 :: states, actions⟩)
-          : IsPostfixFragment ⟨state0 :: states, actions⟩
+          : IsSuffixFragment ⟨state0 :: states, actions⟩
+
+
+structure PrefixFragment (ts: TransitionSystem) where
+  raw: ts.FiniteExecutionFragmentRaw
+  is_valid: IsPrefixFragment raw
+
+structure SuffixFragment (ts: TransitionSystem) where
+  raw: ts.FiniteExecutionFragmentRaw
+  is_valid: IsSuffixFragment raw
 
 end FiniteExecutionFragmentRaw
 
@@ -31,7 +40,7 @@ inductive IsExpr {ts: TransitionSystem} : ExprRaw ts → Prop where
   | finite1 (total: ts.FiniteExecutionFragmentRaw) (req: ts.IsFiniteExecutionFragment total)
             : IsExpr (.finite1 total)
   | finite2 (pre: ts.FiniteExecutionFragmentRaw) (post: ts.FiniteExecutionFragmentRaw)
-            (req1: pre.IsPrefixFragment) (req2: post.IsPostfixFragment)
+            (req1: pre.IsPrefixFragment) (req2: post.IsSuffixFragment)
             : IsExpr (.finite2 pre post)
   | infinite1 (pre: ts.FiniteExecutionFragmentRaw) (req: pre.IsPrefixFragment)
             : IsExpr (.infinite1 pre)
@@ -42,19 +51,60 @@ structure Expr (ts: TransitionSystem) where
   is_valid: IsExpr raw
 
 
-namespace Expr
+namespace ExprRaw
 
 variable {ts: TransitionSystem}
+
+open FiniteExecutionFragmentRaw
 
 /-
 inductive Mem : ts.ExecutionFragment → Expr ts → Prop where
   | finite1 (ef: ts.FiniteExecutionFragment)
             : Mem (.ofFinite ef) ⟨.finite1 ef.raw, .finite1 ef.raw ef.is_valid⟩
-  |
+  | finite2 (ef: ts.FiniteExecutionFragment) (pre: PrefixFragment ts) (post: SuffixFragment ts)
+            (req1: ExecutionFragmentRaw.IsPrefix pre.raw (.finite ef.raw))
+            (req2: ExecutionFragmentRaw.IsSuffix post.raw (.finite ef.raw))
+            : Mem (.ofFinite ef) ⟨.finite2 pre.raw post.raw, .finite2 pre.raw post.raw pre.is_valid post.is_valid⟩
+  | infinite1 (ef: ts.InfiniteExecutionFragment) (pre: PrefixFragment ts)
+              (req: ExecutionFragmentRaw.IsPrefix pre.raw (.infinite ef.raw))
+              : Mem (.ofInfinite ef) ⟨.infinite1 pre.raw, .infinite1 pre.raw pre.is_valid⟩
 -/
 
+inductive Mem : ts.ExecutionFragmentRaw → ExprRaw ts → Prop where
+  | finite1 (ef: ts.FiniteExecutionFragment)
+            : Mem (.finite ef.raw) (.finite1 ef.raw)
+  | finite2 (ef: ts.FiniteExecutionFragment) (pre: PrefixFragment ts) (post: SuffixFragment ts)
+            (req1: ExecutionFragmentRaw.IsPrefix pre.raw (.finite ef.raw))
+            (req2: ExecutionFragmentRaw.IsSuffix post.raw (.finite ef.raw))
+            : Mem (.finite ef.raw) (.finite2 pre.raw post.raw)
+  | infinite1 (ef: ts.InfiniteExecutionFragment) (pre: PrefixFragment ts)
+              (req: ExecutionFragmentRaw.IsPrefix pre.raw (.infinite ef.raw))
+              : Mem (.infinite ef.raw) (.infinite1 pre.raw)
 
-end Expr
+theorem mem_imp_isExecutionFragment ef ex (h: @Mem ts ef ex) : ts.IsExecutionFragment ef := by
+  cases h with
+  | finite1 ef =>
+    refine .finite _ ?_
+    exact ef.is_valid
+  | finite2 ef _ _ _ _ =>
+    refine .finite _ ?_
+    exact ef.is_valid
+  | infinite1 ef pre req =>
+    refine .infinite _ ?_
+    exact ef.is_valid
+
+theorem mem_imp_isExpr ef ex (h: @Mem ts ef ex) : IsExpr ex := by
+  cases h with
+  | finite1 ef =>
+    exact .finite1 ef.raw ef.is_valid
+  | finite2 ef pre post _ _ =>
+    exact .finite2 pre.raw post.raw pre.is_valid post.is_valid
+  | infinite1 ef pre _ =>
+    exact .infinite1 pre.raw pre.is_valid
+
+def EvalToSet (ex: ExprRaw ts) : Set ts.ExecutionFragmentRaw := {ef | Mem ef ex}
+
+end ExprRaw
 
 
 
